# baseURI: http://www.tern.org.au/cv/corveg/site-sample-floristics
# imports: http://www.w3.org/2004/02/skos/core
# imports: http://www.w3.org/ns/sosa/

@prefix cv-corveg: <http://www.tern.org.au/cv/corveg/> .
@prefix dct: <http://purl.org/dc/terms/> .
@prefix owl: <http://www.w3.org/2002/07/owl#> .
@prefix rdf: <http://www.w3.org/1999/02/22-rdf-syntax-ns#> .
@prefix rdfs: <http://www.w3.org/2000/01/rdf-schema#> .
@prefix skos: <http://www.w3.org/2004/02/skos/core#> .
@prefix sosa: <http://www.w3.org/ns/sosa/> .
@prefix xsd: <http://www.w3.org/2001/XMLSchema#> .

cv-corveg:site-sample-floristics
  rdf:type owl:Ontology ;
  owl:imports <http://www.w3.org/2004/02/skos/core> ;
  owl:imports sosa: ;
.
cv-corveg:site-sample-floristics-A
  rdf:type skos:Concept ;
  rdf:type sosa:Procedure ;
  skos:definition "Complete list of all species present within the site." ;
  skos:prefLabel "Complete List" ;
  skos:hiddenLabel "1" ;
  skos:notation "A" ;
.
cv-corveg:site-sample-floristics-B
  rdf:type skos:Concept ;
  rdf:type sosa:Procedure ;
  skos:definition "List of all woody species present within the site (trees, shrubs, climbers)." ;
  skos:prefLabel "Woody Species" ;
  skos:hiddenLabel "2" ;
  skos:notation "B" ;
.
cv-corveg:site-sample-floristics-C
  rdf:type skos:Concept ;
  rdf:type sosa:Procedure ;
  skos:definition "Woody species plus perennial herbs (trees, shrubs, climbers plus perennial herbs)." ;
  skos:prefLabel "Woody Species and Perennial Herbs" ;
  skos:hiddenLabel "3" ;
  skos:notation "C" ;
.
cv-corveg:site-sample-floristics-D
  rdf:type skos:Concept ;
  rdf:type sosa:Procedure ;
  skos:definition "Dominant characteristic species only/incomplete record of species presented." ;
  skos:prefLabel "Dominant characteristic species" ;
  skos:hiddenLabel "4" ;
  skos:notation "D" ;
.
cv-corveg:site-sample-floristics-E
  rdf:type skos:Concept ;
  rdf:type sosa:Procedure ;
  skos:definition "Other (project-specific, such as weed survey)." ;
  skos:prefLabel "Other" ;
  skos:hiddenLabel "5" ;
  skos:notation "E" ;
.
cv-corveg:site-sample-floristicss
  rdf:type skos:Collection ;
  skos:prefLabel "Site sample floristics concepts" ;
  skos:member cv-corveg:site-sample-floristics-A ;
  skos:member cv-corveg:site-sample-floristics-B ;
  skos:member cv-corveg:site-sample-floristics-C ;
  skos:member cv-corveg:site-sample-floristics-D ;
  skos:member cv-corveg:site-sample-floristics-E ;
  skos:notation "ssf" ;
.
